examples/wysteria/lib.fst
@@ -1,124 +1,77 @@
 (*--build-config
-    options:--admit_fsi OrdSet --admit_fsi OrdMap --admit_fsi Set --admit_fsi Wysteria;
+    options:--admit_fsi Set --admit_fsi Wysteria;
     variables:LIB=../../lib;
-    other-files:$LIB/ghost.fst $LIB/ext.fst $LIB/set.fsi $LIB/ordset.fsi $LIB/ordmap.fsi $LIB/heap.fst $LIB/st.fst $LIB/list.fst wysteria.fsi
+    other-files:$LIB/ghost.fst $LIB/ext.fst $LIB/set.fsi $LIB/heap.fst $LIB/st.fst $LIB/all.fst wysteria.fsi
  --*)
 
 module WLib
 
-open OrdMap
-open OrdSet
-
 open Wysteria
-
-val wfold_helper: #a:Type -> #b:Type -> #req_f:(mode -> Type) -> #ens_f:(mode -> a -> Type)
-                  -> w:Wire b
-                  -> =f:(a -> (p:prin{w_contains p w}) -> x:b{w_select p w = x} -> Wys a req_f ens_f)
-                  -> a
-                  -> ps:eprins{forall p. mem p ps ==> w_contains p w}
-                  -> Wys a (fun m0 -> Mode.m m0 = Sec                                 /\
-                                      (forall y. mem y ps ==> CanProjWireS #b m0 w y) /\
-                                      req_f m0)
-                           (fun m0 r -> True)
-let rec wfold_helper w f x ps =
-  if ps = empty then x
-  else
-    let Some p = choose ps in
-    let y = projwire_s w p in
-    wfold_helper w f (f x p y) (remove p ps)
 
 (*
  * mode should be able to project all values from the wire bundle
  *)
-type wfold_pre (#b:Type) (m:mode) (w:Wire b) =
-  (forall p. w_contains p w ==> CanProjWireS #b m w p)
+type wfold_pre (#b:Type) (m:mode) (ps:eprins) (w:Wire b) =
+  Mode.m m = Sec /\ (forall p. mem p ps ==> (w_contains p w /\ CanProjWireS #b m w p))
 
+(* we can give a more precise type to p arg of f, p:prin{mem p ps}, but then unification in the recursive call fails *)
 val wfold: #a:Type -> #b:Type -> #req_f:(mode -> Type) -> #ens_f:(mode -> a -> Type)
-           -> w:Wire b
+           -> ps:eprins
+           -> w:Wire b{forall p. mem p ps ==> w_contains p w}
            -> =f:(a -> (p:prin{w_contains p w}) -> x:b{w_select p w = x} -> Wys a req_f ens_f)
            -> a
-           -> Wys a (fun m0   -> Mode.m m0 = Sec /\ wfold_pre m0 w /\ req_f m0)
-                    (fun m0 r -> True)
-let wfold w f x =
-  let ps = w_dom w in
-  wfold_helper w f x ps
-
-val waps_helper: #a:Type -> #b:Type -> #req_f:(mode -> Type) -> #ens_f:(mode -> b -> Type)
-                 -> w:Wire a
-                 -> =f:(p:prin{w_contains p w} -> x:a{w_select p w = x} -> Wys b req_f ens_f)
-                 -> ps:eprins{forall p. mem p ps ==> w_contains p w}
-                 -> Wys (Wire b) (fun m0 -> Mode.m m0 = Sec                                        /\
-                                            (forall y. mem y ps ==> CanProjWireS #a m0 w y)        /\
-                                            (forall y. mem y ps ==> CanMkWireS b m0 (singleton y)) /\
-                                            req_f m0)
-                                 (fun m0 r -> b2t (w_dom r = ps))
-let rec waps_helper (#a:Type) (#b:Type) (#req_f:mode -> Type) (#ens_f:mode -> b -> Type) w f ps =
-  if ps = empty then w_empty
+           -> Wys a (fun m0 -> wfold_pre #b m0 ps w /\ req_f m0) (fun m0 r -> True)
+              (decreases (size ps))
+let rec wfold ps w f x =
+  if ps = empty then x
   else
-    let Some p = choose ps in
+    let p = choose ps in
     let y = projwire_s w p in
-    let wp = mkwire_s (singleton p) (f p y) in
-    let ps_rest = remove p ps in
-    let w' = waps_helper #a #b #req_f #ens_f w f ps_rest in
-    w_concat wp w'
+    wfold (remove p ps) w f (f x p y)
+
+type waps_pre (#a:Type) (#b:Type) (m:mode) (ps:eprins) (w:Wire a) =
+  Mode.m m = Sec /\ (forall p. mem p ps ==> (w_contains p w /\ CanProjWireS #a m w p /\ CanMkWireS b m (singleton p)))
 
 val waps: #a:Type -> #b:Type -> #req_f:(mode -> Type) -> #ens_f:(mode -> b -> Type)
-          -> w:Wire a
+          -> ps:prins
+          -> w:Wire a{forall p. mem p ps ==> w_contains p w}
           -> =f:(p:prin{w_contains p w} -> x:a{w_select p w = x} -> Wys b req_f ens_f)
-          -> Wys (Wire b) (fun m0 -> Mode.m m0 = Sec                                        /\
-                                     (forall y. w_contains y w ==> CanProjWireS #a m0 w y)        /\
-                                     (forall y. w_contains y w ==> CanMkWireS b m0 (singleton y)) /\
-                                     req_f m0)
-                          (fun m0 r -> True)
-let rec waps w f =
-  let ps = w_dom w in
-  waps_helper w f ps
+          -> Wys (Wire b) (fun m0 -> waps_pre #a #b m0 ps w /\ req_f m0)
+                          (fun m0 r -> b2t (w_dom r = ps))
+             (decreases (size ps))
+let rec waps ps w f =
+  let p = choose ps in
+  let ps' = remove p ps in
+  let y = projwire_s w p in
+  let wp = mkwire_s (singleton p) (f p y) in
+  if ps' = empty then wp
+  else
+    let w' = waps ps' w f in
+    concat_wire wp w'
 
-(*val wapp_helper: #a:Type -> #b:Type -> #req_f:(mode -> Type) -> #ens_f:(mode -> b -> Type)
-                 -> w:Wire a
-                 -> =f:(p:prin{contains w p} -> x:a{sel w p = x} -> Wys b req_f ens_f)
-                 -> l:list prin
-                 -> Wys (Wire b) (fun m0 -> (forall p. List.mem p l ==> contains w p) /\
-                                            (forall p. contains w p ==> (DelPar m0 (singleton p) /\
-                                                                         req_f (Mode Par (singleton p)))))
-                                 (fun m0 r -> True)
-let rec wapp_helper 'a 'b 'r 'e w f l =
-  match l with
-    | []     -> empty_wire
-    | hd::tl ->
-      let g: p:prin{contains w p} -> Wys 'b (fun m0 -> b2t (m0 = Mode Par (singleton p))) (fun m0 r -> True) =
-        fun p ->
-          let x = projwire_p w p in
-          f p x
-      in
-      empty_wire
-
-      (*
-       * we would like to not pass all arguments to g.
-       * but writing this fails and gives an error:
-         let g: #b:Type -> (p:prin{contains w p}) ->
-                           Wys b (fun m0 -> b2t (m0 = Mode Par (singleton p)))
-       *)
-      (*let g: #a:Type -> #b:Type -> #req_f:(mode -> Type) -> #ens_f:(mode -> b -> Type)
-             -> w:Wire a
-             -> =f:(p:prin{contains w p} -> x:a{sel w p = x} -> Wys b req_f ens_f)
-             -> (p:prin{contains w p})
-             -> unit
-             -> Wys b (fun m0 -> m0 = Mode Par (singleton p) /\ req_f m0) (fun m0 r -> True) =
-        fun w f p _ ->
-          let x = projwire_p w p in
-          f p x
-      in*)
-
-      (*let w1 = wapp_helper w f tl in
-      let x = as_par (singleton hd) (g w f hd) in //error here: expected type unit -> Wys b, got unit -> Wys b
-      let w2 = mkwire_p (singleton hd) x in
-      concat_wire w1 w2*)
+type wapp_pre (#a:Type) (#b:Type) (m:mode) (ps:eprins) (w:Wire a) (req_f: mode -> Type) =
+  (forall p. mem p ps ==> (w_contains p w /\ DelPar m (singleton p)   /\
+                           CanMkWireP b m (singleton p) (singleton p) /\
+                           req_f (Mode Par (singleton p))))
 
 val wapp: #a:Type -> #b:Type -> #req_f:(mode -> Type) -> #ens_f:(mode -> b -> Type)
-                     -> w:Wire a
-                     -> =f:(p:prin{contains w p} -> x:a{sel w p = x} -> Wys b req_f ens_f)
-                     -> Wys (Wire b) (fun m0   -> (forall p. contains w p ==> (DelPar m0 (singleton p) /\
-                                                                               req_f (Mode Par (singleton p)))))
-                                     (fun m0 r -> True)
-let wapp w f = wapp_helper w f (dom_of_wire w)*)
+          -> ps:prins
+          -> w:Wire a{forall p. mem p ps ==> w_contains p w}
+          -> =f:(p:prin{w_contains p w} -> x:a{w_select p w = x} -> Wys b req_f ens_f)
+          -> Wys (Wire b) (fun m0 -> wapp_pre #a #b m0 ps w req_f)
+                          (fun m0 r -> b2t (w_dom r = ps))
+             (decreases (size ps))
+let rec wapp 'a 'b 'req_f 'ens_f ps w f =
+  let g: p:prin{mem p ps} -> unit -> Wys 'b (fun m0 -> m0 = Mode Par (singleton p) /\ 'req_f m0) (fun m0 r -> True) =
+    fun p _ ->
+      let x = projwire_p w p in
+      f p x
+  in
+  let p = choose ps in
+  let ps' = remove p ps in
+  let py = as_par (singleton p) (g p) in
+  let wp = mkwire_p #'b #(singleton p) (singleton p) py in
+  if ps' = empty then wp
+  else
+    let w' = wapp (remove p ps) w f in
+    concat_wire wp w'
