examples/wysteria/mill4.fst
@@ -1,0 +1,48 @@
+(*--build-config
+    options:--admit_fsi Set --admit_fsi Wysteria;
+    variables:LIB=../../lib;
+    other-files:$LIB/ghost.fst $LIB/ext.fst $LIB/set.fsi $LIB/heap.fst $LIB/st.fst $LIB/all.fst wysteria.fsi
+ --*)
+
+(* Millionaire's for any 2 parties, private output for the first party *)
+
+module SMC
+
+open Wysteria
+
+let alice_s = singleton alice
+let bob_s = singleton bob
+let charlie_s = singleton charlie
+let ab = union alice_s bob_s
+let bc = union bob_s charlie_s
+let abc = union ab charlie_s
+
+type pre  (m:mode)  = fun m0 -> b2t (m0 = m)
+type post (#a:Type) = fun (m:mode) (x:a) -> True
+
+val mill3_sec: #p1:prin -> #p2:prin
+               -> x:Box nat (singleton p1) -> y:Box nat (singleton p2)
+               -> unit
+               -> Wys (Box bool (singleton p1)) (pre (Mode Par (union (singleton p1) (singleton p2)))) post
+let mill3_sec #p1 #p2 x y _ =
+  let s = union (singleton p1) (singleton p2) in
+  let g:unit -> Wys (Box bool (singleton p1)) (pre (Mode Sec s)) post =
+   fun _ ->
+    let r =  (unbox_s x) > (unbox_s y) in
+    box r (singleton p1)
+  in
+  as_sec s g
+
+val mill3: unit -> Wys bool (pre (Mode Par abc)) post
+let mill3 _ =
+  let x = as_par alice_s (read #nat) in
+  let y = as_par bob_s (read #nat) in
+  let z = as_par charlie_s (read #nat) in
+
+  let _ = as_par ab (mill3_sec #alice #bob x y) in
+  let _ = as_par bc (mill3_sec #bob #charlie y z) in
+
+  true
+;;
+
+let _ = main abc mill3 in ()
